remove ps0; comments

src/b_params/Params.thy
@@ -29,6 +29,49 @@ round many parameters individually, we package them up as follows. *)
 
 (* FIXME ops and params are different kinds of things *)
 
+record ('k,'v,'r,'t) store_ops =
+  store_read :: "('r \<Rightarrow> (('k,'v,'r) frame,'t) MM)"
+  store_alloc :: "(('k,'v,'r) frame \<Rightarrow> ('r,'t) MM)"
+  store_free :: "('r list \<Rightarrow> (unit,'t) MM)"
+
+(* FIXME pass store_ops explicitly ? *)
+
+
+datatype ('k,'v,'r,'t) ps1 = Ps1 "constants * 'k ord * ('k,'v,'r,'t) store_ops"
+
+definition dest_ps1 :: "('k,'v,'r,'t) ps1 \<Rightarrow> constants * 'k ord * ('k,'v,'r,'t) store_ops" where
+"dest_ps1 ps1 = (case ps1 of Ps1 (x,y,z) \<Rightarrow> (x,y,z))"
+
+(* NOTE dot_xxx are named after record projections *)
+
+(* FIXME the following just lifts the ps0 projections, and is confusing *)
+(* FIXME cs is normally reserved as a var *)
+definition dot_constants :: "('k,'v,'r,'t) ps1 \<Rightarrow> constants" where
+"dot_constants ps1 = ps1 |> dest_ps1 |> (% (x,y,z). x)"
+
+definition dot_cmp :: "('k,'v,'r,'t) ps1 \<Rightarrow> 'k ord" where
+"dot_cmp ps1 = ps1 |> dest_ps1 |> (% (x,y,z). y)"
+
+definition dot_store_ops :: "('k,'v,'r,'t) ps1 \<Rightarrow> ('k,'v,'r,'t) store_ops" where
+"dot_store_ops ps1 = ps1 |> dest_ps1 |> (% (x,y,z). z)"
+
+
+
+end
+
+
+
+
+
+(*
+definition ps1_ps0' :: "('k,'v,'r,'t) ps1 \<Rightarrow> 'k ps0" where
+"ps1_ps0' ps1 = (ps1|>dest_ps1|>fst)"
+*)
+
+
+
+
+(*
 datatype 'k ps0 = Ps0 "constants * 'k ord"
 
 definition dest_ps0 :: "'k ps0 \<Rightarrow> constants * 'k ord" where
@@ -39,27 +82,5 @@ definition ps0_cs :: "'k ps0 \<Rightarrow> constants" where
 
 definition ps0_cmp_k:: "'k ps0 \<Rightarrow> 'k ord" where 
 "ps0_cmp_k ps0 = (ps0|>dest_ps0|>snd)"
+*)
 
-record ('k,'v,'r,'t) store_ops =
-  store_read :: "('r \<Rightarrow> (('k,'v,'r) frame,'t) MM)"
-  store_alloc :: "(('k,'v,'r) frame \<Rightarrow> ('r,'t) MM)"
-  store_free :: "('r list \<Rightarrow> (unit,'t) MM)"
-
-datatype ('k,'v,'r,'t) ps1 = Ps1 "'k ps0 * ('k,'v,'r,'t) store_ops"
-
-definition dest_ps1 :: "('k,'v,'r,'t) ps1 \<Rightarrow> 'k ps0 * ('k,'v,'r,'t) store_ops" where
-"dest_ps1 ps1 = (case ps1 of Ps1 (x,y) \<Rightarrow> (x,y))"
-
-definition ps1_ps0 :: "('k,'v,'r,'t) ps1 \<Rightarrow> 'k ps0" where
-"ps1_ps0 ps1 = (ps1|>dest_ps1|>fst)"
-
-definition ps1_store_ops :: "('k,'v,'r,'t) ps1 \<Rightarrow> ('k,'v,'r,'t) store_ops" where
-"ps1_store_ops ps1 = (ps1 |> dest_ps1 |> snd)"
-
-definition cs :: "('k,'v,'r,'t) ps1 \<Rightarrow> constants" where
-"cs ps1 = ps1 |> dest_ps1 |> fst |> ps0_cs"
-
-definition cmp_k :: "('k,'v,'r,'t) ps1 \<Rightarrow> 'k ord" where
-"cmp_k ps1 = ps1 |> dest_ps1 |> fst |> ps0_cmp_k"
-
-end
