src/a_tree/Tree_stack.thy
@@ -24,12 +24,13 @@ record ('k,'a) ts_frame =
   f_ts2 :: "'a list"
   
 
-definition dest_ts_frame :: "('k,'a) ts_frame \<Rightarrow> ('k list * 'a list) * 'a * ('k list * 'a list)" where
+definition dest_ts_frame :: 
+  "('k,'a) ts_frame \<Rightarrow> ('k list * 'a list) * 'a * ('k list * 'a list)" 
+where
 "dest_ts_frame f = (
   (f|>f_ks1,f|>f_ts1),
   f|>f_t,
-  (f|>f_ks2, f|>f_ts2)
-)"
+  (f|>f_ks2, f|>f_ts2))"
 
 
 definition ts_frame_map :: "('a \<Rightarrow> 'b) \<Rightarrow> ('k,'a) ts_frame \<Rightarrow> ('k,'b) ts_frame" where
@@ -40,8 +41,7 @@ definition ts_frame_map :: "('a \<Rightarrow> 'b) \<Rightarrow> ('k,'a) ts_frame
     f_t=(f|>f_t|>g),
     f_ks2=(f|>f_ks2),
     f_ts2=(f|>f_ts2|>List.map g)
-  \<rparr>
-)"
+  \<rparr>)"
 
 
 definition with_t :: "'a \<Rightarrow> ('k,'a) ts_frame \<Rightarrow> ('k,'a) ts_frame" where
@@ -57,21 +57,22 @@ definition ts_frame_equal:: "('k,'a) ts_frame \<Rightarrow> ('k,'a) ts_frame \<R
 (* FIXME rename to stack *)
 type_synonym ('k,'a) ts_frames = "('k,'a) ts_frame list"   
 
+(* map a function over the non-'k component *)
 definition stack_map :: "('a \<Rightarrow> 'b) \<Rightarrow> ('k,'a) ts_frame list \<Rightarrow> ('k,'b) ts_frame list" where
 "stack_map f stk = (
-  stk |> List.map (ts_frame_map f)
-)"
+  stk |> List.map (ts_frame_map f))"
 
 definition stack_equal :: "('k,'a) ts_frames \<Rightarrow> ('k,'a) ts_frames \<Rightarrow> bool" where
 "stack_equal s1 s2 = failwith (STR ''FIXME patch'')"
 
-
+(* a tree_stack has 'a = ('k,'v)tree *)
 type_synonym ('k,'v) tree_stack = "('k,('k,'v)tree) ts_frames"
 
 
 
-(* get bounds ------------------------------------------------------- *)
+(* stack_to_lu_of_child (get bounds of focus) ---------------------------------- *)
 
+(* get the bound surrounding the focus *)
 primrec stack_to_lu_of_child :: "('k,'a) ts_frames \<Rightarrow> 'k option * 'k option" where
 "stack_to_lu_of_child [] = (None,None)"
 | "stack_to_lu_of_child (x#stk') = (
@@ -79,15 +80,16 @@ primrec stack_to_lu_of_child :: "('k,'a) ts_frames \<Rightarrow> 'k option * 'k 
     let (ks1,ks2) = (x|>f_ks1,x|>f_ks2) in    
     let l = (if ks1 \<noteq> [] then Some(ks1|>List.last) else l') in
     let u = (if ks2 \<noteq> [] then Some(ks2|>List.hd) else u') in
-    (l,u)
-  )"
+    (l,u))"
 
 
 
-(* convert to/from tree from/to tree stack -------------------------- *)
+(* tree_to_stack, stack_to_tree, no_focus -------------------------- *)
 
 (* the n argument ensures the stack has length n; we assume we only call this with n\<le>height t *)
-primrec tree_to_stack :: "'k ord \<Rightarrow> 'k \<Rightarrow> ('k,'v)tree \<Rightarrow> nat \<Rightarrow> (('k,'v)tree * ('k,'v)tree_stack)" where
+primrec tree_to_stack :: 
+  "'k ord \<Rightarrow> 'k \<Rightarrow> ('k,'v)tree \<Rightarrow> nat \<Rightarrow> (('k,'v)tree * ('k,'v)tree_stack)" 
+where
 "tree_to_stack ord k t 0 = (t,[])"
 | "tree_to_stack ord k t (Suc n) = (
     let (fo,stk) = tree_to_stack ord k t n in
@@ -98,7 +100,7 @@ primrec tree_to_stack :: "'k ord \<Rightarrow> 'k \<Rightarrow> ('k,'v)tree \<Ri
       let frm = \<lparr>f_ks1=ks1,f_ts1=ts1,f_t=t',f_ks2=ks2,f_ts2=ts2\<rparr> in
       (t',frm#stk) ))"
 
-(* we may provide a new focus *)
+(* when converting a stack to a tree we may provide a new focus *)
 fun stack_to_tree :: "('k,'v)tree \<Rightarrow> ('k,'v)tree_stack \<Rightarrow> ('k,'v)tree" where
 "stack_to_tree fo ts = (
   case ts of 
@@ -108,7 +110,7 @@ fun stack_to_tree :: "('k,'v)tree \<Rightarrow> ('k,'v)tree_stack \<Rightarrow> 
     let fo' = Node(ks1@ks2,ts1@[fo]@ts2) in
     stack_to_tree fo' ts' ))"
 
-(* remove "focus" *)
+(* remove "focus"; NOTE 'a option is always None FIXME so why not use unit? *)
 definition no_focus :: "('k,'a) ts_frames \<Rightarrow> ('k,'a option) ts_frames" where
 "no_focus stk = (
   stk |> stack_map Some |> (% stk. 
@@ -116,17 +118,17 @@ definition no_focus :: "('k,'a) ts_frames \<Rightarrow> ('k,'a option) ts_frames
 
 
 
-(* add new stk ts_frame --------------------------------------------- *)
+(* add_new_stk_frame; r_stk_to_rs --------------------------------------------- *)
 
 definition add_new_stack_frame :: 
-  "'k ord => 'k \<Rightarrow> ('k list * 'a list) \<Rightarrow> ('k,'a) ts_frames \<Rightarrow> (('k,'a) ts_frames * 'a)" where
+  "'k ord => 'k \<Rightarrow> ('k list * 'a list) \<Rightarrow> ('k,'a) ts_frames \<Rightarrow> (('k,'a) ts_frames * 'a)" 
+where
 "add_new_stack_frame cmp k ks_rs stk = (
   let (ks,rs) = ks_rs in
   let ((ks1,rs1),r',(ks2,rs2)) = split_ks_rs cmp k (ks,rs) in
   (* let (l,u) = stack_to_lu_of_child stk in *)
   let frm' = \<lparr>f_ks1=ks1,f_ts1=rs1,f_t=r', f_ks2=ks2,f_ts2=rs2 \<rparr> in
-  (frm'#stk,r')
-)"
+  (frm'#stk,r') )"  (* FIXME why return r' explicitly? why not get from f_t? *)
 
 
 definition r_stk_to_rs :: "('k,'r) ts_frame list \<Rightarrow> 'r list" where 
