src/b_params/Pre_params.thy
@@ -13,7 +13,7 @@ type_synonym ('k,'v,'r,'t) r2f = "('t \<Rightarrow> 'r \<Rightarrow> ('k,'v,'r) 
 
 type_synonym ('k,'v,'r,'t) r2t = "('t \<Rightarrow> 'r \<Rightarrow> ('k,'v) tree option)"
 
-
+(* n is fuel (the height of the tree); t is not needed FIXME? *)
 fun mk_r2t' :: "('k,'v,'r,'t) r2f \<Rightarrow> nat \<Rightarrow> ('k,'v,'r,'t) r2t" where
 "mk_r2t' r2f n t r = (
   case n of 
@@ -28,14 +28,9 @@ fun mk_r2t' :: "('k,'v,'r,'t) r2f \<Rightarrow> nat \<Rightarrow> ('k,'v,'r,'t) 
         let ts = List.map (mk_r2t' r2f n t) rs in
         case (List.filter is_None ts) of
         [] \<Rightarrow> Some(Node(ks,ts|>List.map dest_Some))
-        | _ \<Rightarrow> None
-      )
-    )
-  )
-)"
+        | _ \<Rightarrow> None ))))"
 
 (* map a blocks-and-pointers tree to an ADT tree *)
-
 definition mk_r2t :: "('k,'v,'r,'t) r2f \<Rightarrow> nat \<Rightarrow> ('k,'v,'r,'t) r2t" where
 "mk_r2t = mk_r2t'"
 
